src/fresh/relabels/freefresh.v
@@ -1,41 +1,12 @@
-Implicit Type X: Type.
+From FreeMonad Require Export FreeMonad.
 
-Inductive Free (SIG : Type -> Type) X :=
-| ret : X -> Free SIG X
-| op : forall Y, SIG Y -> (Y -> Free SIG X) -> Free SIG X.
-
-Arguments ret [SIG X] _.
-Arguments op [SIG X Y].
-
-Section Bind.
-  Variable X Y : Type.
-  Variable SIG : Type -> Type.
-  (* =bind= *)
-  Fixpoint bind (m: Free SIG X)(f: X -> Free SIG Y): Free SIG Y :=
-  match m with
-  | ret v => f v
-  | op e k => op e (fun n => bind (k n) f)
-  end.
-(* =end= *)
-End Bind.
-
-Arguments bind [_][_] [_] m f.
-
-(* =FreeFresh= *)
 Inductive Fresh : Type -> Type :=
 | gensymOp : unit -> Fresh nat.
-(* =end= *)
 
-(* =fresh= *)
-Definition gensym (tt: unit): Free Fresh nat := op (gensymOp tt) (@ret Fresh nat).
-(* =end= *)
-
-Notation "'do' x '<-' e1 ';' e2" :=
-  (bind e1 (fun x => e2)) (x name, at level 50).
+Definition gensym (tt: unit): Free Fresh nat := syntax_effect (gensymOp tt).
 
 Require Import tree.
 
-(* =label= *)
 Fixpoint label {X} (t : Tree X) : Free Fresh (Tree nat):=
   match t with
   | Leaf _ =>
@@ -46,4 +17,3 @@ Fixpoint label {X} (t : Tree X) : Free Fresh (Tree nat):=
     do r <- label r;
     ret (Node l r)
   end.
-(* =end= *)
