src/lib/FM/FreeMonad.v
@@ -1,0 +1,58 @@
+Require Import FunctionalExtensionality.
+
+Inductive Free (SIG : Type -> Type) X :=
+| ret : X -> Free SIG X
+| op : forall Y, SIG Y -> (Y -> Free SIG X) -> Free SIG X.
+
+Arguments ret [SIG X] _.
+Arguments op [SIG X Y].
+
+Fixpoint bind {SIG X Y} (m: Free SIG X)(f: X -> Free SIG Y): Free SIG Y :=
+  match m with
+  | ret v => f v
+  | op e k => op e (fun n => bind (k n) f)
+  end.
+
+Arguments bind [_][_] [_] m f.
+
+Definition syntax_effect {SIG X} (m : SIG X) : Free SIG X := op m (@ret SIG X).
+
+Definition bind2 {SIG} {A B C: Type} (x: Free SIG (A * B)) (f: A -> B -> Free SIG C) : Free SIG C :=
+  bind x (fun p => f (fst p) (snd p)).
+
+Declare Scope free_monad_scope.
+
+Notation "'ret!' v" := (ret v) (v name, at level 90) : free_monad_scope.
+
+Notation "'do' X <- A ; B" := (bind A (fun X => B))
+   (at level 200, X ident, A at level 100, B at level 200) : free_monad_scope.
+
+Notation "'do' ( X , Y ) <- A ; B" := (bind2 A (fun X Y => B))
+   (at level 200, X ident, Y ident, A at level 100, B at level 200) : free_monad_scope.
+
+Notation "'let!' x ':=' e1 'in' e2" :=
+  (bind e1 (fun x => e2)) (x name, at level 50) : free_monad_scope.
+
+Notation "'let!' ( X , Y ) ':=' A 'in' B" := (bind2 A (fun X Y => B))
+     (at level 50, X name, Y name): free_monad_scope.
+
+Lemma lid : forall SIG X Y (a : X) (f : X -> Free SIG Y), bind (ret a) f = f a.
+Proof. auto. Qed.
+
+Lemma rid : forall SIG X (m : Free SIG X), bind m (@ret SIG X) = m.
+Proof.
+  fix IH 3.
+  destruct m.
+  reflexivity.
+  simpl. do 2 f_equal.
+  apply functional_extensionality. intro. apply IH.
+Qed.
+
+Lemma assoc_bind : forall SIG X Y Z (m : Free SIG X) f (g : Y -> Free SIG Z),
+    bind (bind m f) g = bind m (fun x => bind (f x) g).
+Proof.
+  fix IH 5.
+  destruct m; intros.
+  reflexivity.
+  simpl. do 2 f_equal. apply functional_extensionality. intro. apply IH.
+Qed.
